# Lagrange multiplier

We want to maximise, or optimise, $f(x)$ subject to: $g(x) = 0$:

$$
\mathcal{L}(x, \alpha) = f(x) - \alpha g(x)
$$

### Example

Consider $f(x,y) = x + y$, subject to $g(x, y): x^2 + y^2 - 1 = 0$

1. Form $\mathcal{L}(x_1, \ldots, x_{n}, \lambda)$ where $\lambda$ is the
   Lagrange multiplier. Then $\mathcal{L} = f + \lambda g$
2. $\nabla \mathcal{L} = (\frac{\partial f}{\partial x_1}, \ldots, \frac{\partial f}{\partial x_n}, \frac{\partial f}{\partial \lambda})$
3. Set $\nabla \mathcal{L} = 0$ and solve for $x_i,\lambda$

So, $\mathcal{L}(x, y, \lambda) = x + y + \lambda(x^2 + y^2 - 1)$

Therefore

$$
\nabla \mathcal{L}(x, y, \lambda) = \begin{bmatrix} 
1 + 2 \lambda x \\
1 + 2 \lambda y \\
x^2 + y^2 - 1
\end{bmatrix} 
$$

Setting $1 + 2 \lambda x = 0$ gives us $x = \frac{-1}{2 \lambda}$

Further, $1 + 2 \lambda y = 0$ gives us $y = \frac{-1}{2 \lambda}$

Substituting back

$$
\begin{align*}
\left( -\frac{1}{2 \lambda} \right)^2 + 
\left( -\frac{1}{2 \lambda} \right)^2 -
1 &= 0 \\[0.5em]
\Rarr \lambda &= \pm \frac{1}{\sqrt{2}}
\end{align*}
$$

### Example 2

$f(x,y,z) = x^2 + 2y - z^2$

$g_1(x,y,z) := 2x - y = 0$

$g_2(x,y,z) := y + z = 0$

Step 1.

$$
\mathcal{L}(x,y,z,\lambda_1,\lambda_2) = x^2 + 2y - z^2 + \lambda_1(2x - y) +
\lambda_2(y + z)
$$

Step 2.

$$
\nabla \mathcal{L} = \begin{bmatrix} 
2x + 2\lambda_1 \\
2 - \lambda_1 + \lambda_2 \\
-2z + \lambda_2 \\
2x - y \\
y + z
\end{bmatrix}
$$

Setting row 0 to 0 gives $x = -\lambda_1$

Setting row 2 to 0 gives $z = \lambda_2 / 2$

Setting row 3 to 0 gives $y = 2x$

$$
\begin{align*}
y &= -2\lambda_1 \\[0.5em]
x &= -\lambda_1 \\[0.5em]
z &= \frac{\lambda_2}{2} \Rarr z = 2\lambda_2 \\[0.5em]
\end{align*}
$$

This gives us

$$
\begin{align*}
\lambda_2 &= 4\lambda_1 \\[0.5em]
\lambda_1 &= 2/3, \lambda_2 = 2/3 \\[0.5em]
x &= 2/3, y = 4/3, z = -4/3
\end{align*}
$$

Note that these numbers might not be totally accurate.
