# Chain rule

In essence, it's about multiplying gradients:

$$
\frac{dy}{dx} = \frac{dy}{du} \cdot \frac{du}{dx}
$$

Or

$$
(f \circ g)' = (f' \circ g) \times g'
$$

Or

$$
\left[ f(g(x)) \right]' = f'(g(x)) \times g'(x)
$$

Can go deeper:

$$
\left[ f(g(h(x))) \right]' = f'(g(h(x))) \times g'(h(x)) \times h'(x)
$$

### Example

$$
\frac{d}{dx} \exp(\sin(x))
$$

Taking $g(x) = \sin(x)$ and $f(x) = \exp(g(x))$, we have

$$
\begin{align*}
f'(x) &= \exp(g(x)) \\[0.5em]
g'(x) &= \cos(x) \\[0.5em]
\Rarr \frac{d}{dx} \exp(\sin(x)) &= \cos(x) \exp(\sin(x)) \\[0.5em]
\end{align*}
$$
